test/collection_positivity.lean
@@ -1,0 +1,24 @@
+import Std.Data.HashMap
+import Std.Data.RBMap
+
+/-!
+# Positivity tests
+
+Here we test that it is possible to write inductive types which contain a collection that contains
+the type being defined.
+
+-/
+
+open Std
+
+inductive ContainsItselfInAssocListValues where
+  | base
+  | recursive (l : AssocList Bool ContainsItselfInAssocListValues)
+
+inductive ContainsItselfInHashMapValues where
+  | base
+  | recursive (l : HashMap.Imp Bool ContainsItselfInHashMapValues)
+
+inductive ContainsItselfInRBMapValues where
+  | base
+  | recursive (l : RBNode (Nat × ContainsItselfInRBMapValues))
